Test/civl/inductive-sequentialization/snapshot-scatter-gather.bpl
@@ -10,7 +10,7 @@ datatype StampedValue {
 } 
 
 datatype Permission {
-    Permission(t_id: Tid, mem_index: int)
+    Permission(tid: Tid, mem_index: int)
 }
 
 const n: int;
@@ -18,20 +18,11 @@ axiom n >= 1;
 
 var {:layer 0,2} mem: [int]StampedValue;
 var {:layer 0,2} r1: [Tid][int]StampedValue;  
-var {:layer 0,2} r2: [Tid][int]StampedValue; 
 var {:linear} {:layer 0,2} pSet: Set Permission;
+var {:layer 0,2} channels: [Tid](Option [int]StampedValue);
 
 function {:inline} WholeTidPermission(tid: Tid): Set Permission {
-    Set((lambda {:pool "D"} x: Permission :: x->t_id == tid && (1 <= x->mem_index) && (x->mem_index <= n)))
-}
-
-action {:layer 1} start (tid: Tid)
-modifies pSet;
-creates main_f;
-{
-    var {:linear} sps: Set Permission;
-    call sps := Set_Get(pSet, (lambda x: Permission :: (x->t_id == tid) && (1 <= x->mem_index) && (x->mem_index <= n)));
-    call create_async(main_f(tid, sps));
+    Set((lambda {:pool "D"} x: Permission :: x->tid == tid && (1 <= x->mem_index) && (x->mem_index <= n)))
 }
 
 async action {:layer 1} main_f(tid: Tid, {:linear_in} sps: Set Permission)
@@ -40,32 +31,26 @@ modifies pSet;
 creates read_f;
 {
     assume {:add_to_pool "A", 0, n} true;
-    assert (sps == Set((lambda x: Permission :: (x->t_id == tid) && (1 <= x->mem_index) && (x->mem_index <= n))));
-    call create_asyncs((lambda pa:read_f :: (1 <= pa->perm->val->mem_index) && (pa->perm->val->mem_index <= n) && pa->perm->val->t_id == tid));
+    assert sps == WholeTidPermission(tid);
+    assert channels[tid] == None();
+    call create_asyncs((lambda pa:read_f :: (1 <= pa->perm->val->mem_index) && (pa->perm->val->mem_index <= n) && pa->perm->val->tid == tid));
 }
-
-
 
 action {:layer 2} main_f'(tid: Tid, {:linear_in} sps: Set Permission)
-creates main_s;
-modifies r1, pSet;
+modifies r1, pSet, channels;
 {
-    var {:linear} sps2: Set Permission;
     var {:linear} done_set: Set Permission;
-    sps2 := sps;
     assume {:add_to_pool "A", 0, n} true;
-    assert (sps == Set((lambda x: Permission :: (x->t_id == tid) && (1 <= x->mem_index) && (x->mem_index <= n))));
+    assert sps == WholeTidPermission(tid);
+    assert channels[tid] == None();
     havoc r1;
     assume (forall i:int :: ((1 <= i && i <= n) ==> (r1[tid][i]->ts < mem[i]->ts  || r1[tid][i]== mem[i]))); 
-    call done_set := Set_Get(sps2, (lambda x: Permission :: (x->t_id == tid) && (1 <= x->mem_index) && (x->mem_index <= n))); 
-    call Set_Put(pSet, done_set);
-    call create_async(main_s(tid));
-
+    call Set_Put(pSet, sps);
+    call ChannelSend(tid);
 }
 
-async action {:layer 1} {:exit_condition Set_IsSubset(WholeTidPermission(perm->val->t_id), Set_Add(pSet, perm->val))} read_f({:linear_in} perm: One Permission)
-creates read_f, main_s;
-modifies r1, pSet;
+async action {:layer 1} {:exit_condition Set_IsSubset(WholeTidPermission(perm->val->tid), Set_Add(pSet, perm->val))} read_f({:linear_in} perm: One Permission)
+modifies r1, pSet, channels;
 {
     var {:pool "K"} k:int;
     var {:pool "V"} v:Value;
@@ -75,30 +60,28 @@ modifies r1, pSet;
     if (*) {
         assume {:add_to_pool "K", mem[perm->val->mem_index]->ts, k} {:add_to_pool "V", mem[perm->val->mem_index]->value, v} true;
         assume k < mem[perm->val->mem_index]->ts; 
-        r1[perm->val->t_id][perm->val->mem_index]:= StampedValue(k, v);
+        r1[perm->val->tid][perm->val->mem_index]:= StampedValue(k, v);
     } else {
-        r1[perm->val->t_id][perm->val->mem_index]:= mem[perm->val->mem_index];
+        r1[perm->val->tid][perm->val->mem_index]:= mem[perm->val->mem_index];
     }
     call One_Put(pSet, perm);
 
-    if (Set_IsSubset(WholeTidPermission(perm->val->t_id), pSet)){
-        call create_async(main_s(perm->val->t_id));
+    if (Set_IsSubset(WholeTidPermission(perm->val->tid), pSet)) {
+        call ChannelSend(perm->val->tid);
     }
 }
 
-
-atomic action {: layer 1,2} write(i: int,v: Value)
+atomic action {:layer 1,2} write(i: int,v: Value)
 modifies mem;
 {
     var x: StampedValue;
-
     x := mem[i];
     mem[i] := StampedValue(x->ts + 1, v);
 }
 
 action {:layer 1} Inv_f(tid: Tid, {:linear_in} sps: Set Permission)
-modifies r1, pSet;
-creates read_f, main_s;
+modifies r1, pSet, channels;
+creates read_f;
 {
     var {:pool "A"} j: int;
     var {:linear} sps2: Set Permission;
@@ -106,25 +89,38 @@ creates read_f, main_s;
     var choice: read_f;
     sps2 := sps;
     assert sps == WholeTidPermission(tid);
+    assert channels[tid] == None();
     assume {:add_to_pool "A", 0, j+1, n} 0 <= j && j <= n;
     havoc r1;
     assume (forall i:int :: ((1 <= i && i <= j) ==> (r1[tid][i]->ts < mem[i]->ts || r1[tid][i]== mem[i]))); 
 
     assume {:add_to_pool "D", Permission(tid, n)} true;
-    call done_set := Set_Get(sps2, (lambda {:pool "D" } x: Permission :: (x->t_id == tid) && (1 <= x->mem_index) && (x->mem_index <= j)));
+    call done_set := Set_Get(sps2, (lambda {:pool "D" } x: Permission :: (x->tid == tid) && (1 <= x->mem_index) && (x->mem_index <= j)));
   
     call Set_Put(pSet, done_set);
-    if (j < n){
+    if (j < n) {
         choice := read_f(One(Permission(tid, j+1)));
         assume {:add_to_pool "C", choice} true;
-        call create_asyncs((lambda {:pool "C" } pa:read_f :: ((j+1) <=  pa->perm->val->mem_index) && ( pa->perm->val->mem_index <= n) && pa->perm->val->t_id == tid));
+        call create_asyncs((lambda {:pool "C" } pa:read_f :: j+1 <=  pa->perm->val->mem_index && pa->perm->val->mem_index <= n && pa->perm->val->tid == tid));
         call set_choice(choice);
-    }
-    else{
-        call create_async(main_s(tid));
+    } else {
+        call ChannelSend(tid);
     }
 }
 
-async action {:layer 1,2} main_s(tid: Tid)
+action {:layer 1,2} ChannelSend(tid: Tid)
+modifies channels;
 {
+    assert Set_IsSubset(WholeTidPermission(tid), pSet);
+    assert channels[tid] == None();
+    channels[tid] := Some(r1[tid]);
+}
+
+action {:layer 1,2} ChannelReceive(tid: Tid) returns (r: [int]StampedValue)
+modifies channels;
+{
+    assert Set_IsSubset(WholeTidPermission(tid), pSet);
+    assert channels[tid] != None();
+    r := channels[tid]->t;
+    channels[tid] := None();
 }
